memory_ops_solvers.v
@@ -40,7 +40,7 @@ Module MemoryOpsSolvers.
 Definition mload_solver_type := sstack_val -> smemory -> nat -> smap -> stack_op_instr_map -> smap_value.
 
 Definition mload_solver_ext_type := sstack_val_cmp_ext_1_t -> sstack_val -> smemory -> nat -> smap -> stack_op_instr_map -> smap_value.
-            
+
 Definition mload_solver_valid_res (mload_solver: mload_solver_type) :=
   forall m smem soffset instk_height smv ops,
     valid_smemory instk_height (get_maxidx_smap m) smem -> (* The memory is valid *)
